Coq.Init.Byte lemmas & use it in LittleEndian.v instead of "word 8"

src/coqutil/Word/LittleEndian.v
@@ -3,40 +3,40 @@ Require Import coqutil.Z.Lia.
 Require Import coqutil.Word.Interface coqutil.Datatypes.HList coqutil.Datatypes.PrimitivePair.
 Require Import coqutil.Word.Properties.
 Require Import coqutil.Z.bitblast.
+Require Import coqutil.Byte.
 Local Set Universe Polymorphism.
 
 Local Open Scope Z_scope.
 
 Section LittleEndian.
-  Context {byte: word 8}.
 
   Fixpoint combine (n : nat) : forall (bs : tuple byte n), Z :=
     match n with
     | O => fun _ => 0
-    | S n => fun bs => Z.lor (word.unsigned (pair._1 bs))
+    | S n => fun bs => Z.lor (byte.unsigned (pair._1 bs))
                              (Z.shiftl (combine n (pair._2 bs)) 8)
     end.
 
   Fixpoint split (n : nat) (w : Z) : tuple byte n :=
     match n with
     | O => tt
-    | S n => pair.mk (word.of_Z w) (split n (Z.shiftr w 8))
+    | S n => pair.mk (byte.of_Z w) (split n (Z.shiftr w 8))
     end.
 
-  Lemma combine_split {ok : word.ok byte} (n : nat) (z : Z) :
+  Lemma combine_split (n : nat) (z : Z) :
     combine n (split n z) = z mod 2 ^ (Z.of_nat n * 8).
   Proof.
     revert z; induction n.
     - cbn. intros. rewrite Z.mod_1_r. trivial.
     - cbn [split combine PrimitivePair.pair._1 PrimitivePair.pair._2]; intros.
       erewrite IHn; clear IHn.
-      rewrite word.unsigned_of_Z, Nat2Z.inj_succ, Z.mul_succ_l by blia.
-      unfold word.wrap.
+      rewrite byte.unsigned_of_Z, Nat2Z.inj_succ, Z.mul_succ_l by blia.
+      unfold byte.wrap.
       rewrite <-! Z.land_ones by blia.
       Z.bitblast.
   Qed.
 
-  Lemma split_combine {ok : word.ok byte} (n: nat) bs :
+  Lemma split_combine (n: nat) bs :
     split n (combine n bs) = bs.
   Proof.
     revert bs; induction n.
@@ -44,15 +44,15 @@ Section LittleEndian.
     - destruct bs; cbn [split combine PrimitivePair.pair._1 PrimitivePair.pair._2]; intros.
       specialize (IHn _2).
       f_equal.
-      { eapply Properties.word.unsigned_inj.
-        rewrite word.unsigned_of_Z, <-Properties.word.wrap_unsigned; cbv [word.wrap].
+      { eapply byte.unsigned_inj.
+        rewrite byte.unsigned_of_Z, <-byte.wrap_unsigned; cbv [byte.wrap].
         Z.bitblast; cbn; subst.
         rewrite (Z.testbit_neg_r _ (i-8)) by bomega.
         Z.bitblast_core. }
       { rewrite <-IHn.
         rewrite combine_split.
         f_equal.
-        rewrite <-word.wrap_unsigned.
+        rewrite <-byte.wrap_unsigned; cbv [byte.wrap].
         Z.bitblast; subst; cbn.
         rewrite <-IHn.
         rewrite combine_split.
