src/coqutil/Byte.v
@@ -1,0 +1,106 @@
+Require Coq.Init.Byte Coq.Strings.Byte.
+Require Import Coq.ZArith.ZArith.
+
+Local Open Scope Z_scope.
+
+Notation byte := (Coq.Init.Byte.byte: Type). (* to avoid that some universes are forced to "Set" *)
+
+Module byte.
+  Definition unsigned(b: byte): Z := Z.of_N (Byte.to_N b).
+
+  Definition wrap(z: Z): Z := z mod 2 ^ 8.
+
+  Lemma Byte_of_N_of_mod_not_None: forall z, Byte.of_N (Z.to_N (wrap z)) <> None.
+  Proof.
+    intros z C.
+    apply Byte.of_N_None_iff in C.
+    pose proof (Z.mod_pos_bound z 256 eq_refl) as P.
+    destruct P as [P1 P2].
+    apply Z2N.inj_lt in P2. 3: cbv; discriminate. 2: assumption.
+    apply N.lt_le_pred in P2.
+    simpl in P2.
+    pose proof (N.lt_le_trans _ _ _ C P2) as P3.
+    cbv in P3.
+    discriminate.
+  Qed.
+
+  Definition of_Z(z: Z): byte :=
+    let r := Byte.of_N (Z.to_N (wrap z)) in
+    match r as o return (r = o -> byte) with
+    | Some b => fun _ => b
+    | None => fun E => False_rect byte (Byte_of_N_of_mod_not_None z E)
+    end eq_refl.
+
+  Lemma unsigned_of_Z: forall z, unsigned (of_Z z) = wrap z.
+  Proof.
+    intros. unfold unsigned.
+    pose proof (Z.mod_pos_bound z (2^8) eq_refl) as P.
+    rewrite <- (Z2N.id (wrap z)) by (destruct P; assumption).
+    f_equal.
+    destruct (Byte.of_N (Z.to_N (wrap z))) eqn: E. 2: {
+      apply Byte_of_N_of_mod_not_None in E. contradiction.
+    }
+    erewrite <- (Byte.to_of_N (Z.to_N (wrap z))). 2: exact E.
+    f_equal.
+    unfold of_Z.
+    remember (fun E0 : Byte.of_N (Z.to_N (wrap z)) = None => False_rect byte (Byte_of_N_of_mod_not_None z E0))
+      as F; clear HeqF.
+    revert E F.
+    generalize (Byte.of_N (Z.to_N (wrap z))).
+    clear z P.
+    intros o E.
+    rewrite E.
+    intros.
+    reflexivity.
+  Qed.
+
+  Lemma of_bits_inj: forall bs1 bs2, Byte.of_bits bs1 = Byte.of_bits bs2 -> bs1 = bs2.
+  Proof.
+    intros.
+    rewrite <- (Byte.to_bits_of_bits bs1) in *.
+    rewrite <- (Byte.to_bits_of_bits bs2) in *.
+    do 2 rewrite Byte.of_bits_to_bits in H.
+    f_equal.
+    assumption.
+  Qed.
+
+  Lemma to_bits_inj: forall b1 b2, Byte.to_bits b1 = Byte.to_bits b2 -> b1 = b2.
+  Proof.
+    intros.
+    rewrite <- (Byte.of_bits_to_bits b1) in *.
+    rewrite <- (Byte.of_bits_to_bits b2) in *.
+    do 2 rewrite Byte.to_bits_of_bits in H.
+    f_equal.
+    assumption.
+  Qed.
+
+  Lemma to_N_inj: forall b1 b2, Byte.to_N b1 = Byte.to_N b2 -> b1 = b2.
+  Proof.
+    intros.
+    enough (Some b1 = Some b2). 1: congruence.
+    rewrite <- (Byte.of_to_N b1).
+    rewrite <- (Byte.of_to_N b2).
+    f_equal.
+    assumption.
+  Qed.
+
+  Lemma unsigned_inj: forall b1 b2, unsigned b1 = unsigned b2 -> b1 = b2.
+  Proof.
+    unfold unsigned. intros.
+    apply N2Z.inj in H.
+    apply to_N_inj in H.
+    assumption.
+  Qed.
+
+  Lemma wrap_unsigned: forall x, wrap (unsigned x) = unsigned x.
+  Proof.
+    intros. unfold wrap, unsigned.
+    apply Z.mod_small. split.
+    - apply N2Z.is_nonneg.
+    - change (2 ^ 8) with (Z.of_N (N.succ 255)).
+      apply N2Z.inj_lt.
+      apply N.lt_succ_r.
+      apply (Byte.to_N_bounded x).
+  Qed.
+
+End byte.
